compiler/backend/semantics/dataPropsScript.sml
@@ -193,11 +193,11 @@ QED
 
 val consume_space_with_stack = Q.prove(
   `consume_space x (y with stack := z) = OPTION_MAP (λs. s with stack := z) (consume_space x y)`,
-  EVAL_TAC >> srw_tac[][])
+  EVAL_TAC >> srw_tac[][]);
 
 val consume_space_with_locals = Q.prove(
   `consume_space x (y with locals := z) = OPTION_MAP (λs. s with locals := z) (consume_space x y)`,
-  EVAL_TAC >> srw_tac[][])
+  EVAL_TAC >> srw_tac[][]);
 
 val do_app_with_stack = time Q.prove(
   `do_app op vs (s with stack := z) =
@@ -218,7 +218,7 @@ val do_app_with_stack = time Q.prove(
           rveq >> fs []) >>
           fs[allowed_op_def]>>
           rw [state_component_equality] \\ simp [Once CONJ_COMM] \\
-          rw[EQ_IMP_THM] >> fs[stack_consumed_def,allowed_op_def]
+          rw[EQ_IMP_THM] >> fs[stack_consumed_def,allowed_op_def,PULL_EXISTS]
     );
 
 val do_app_with_stack_and_locals = time Q.prove(
